src/Exec/Exec_DG_Generator.thy
@@ -1,6 +1,6 @@
 theory Exec_DG_Generator
   imports
-    Exec_DG_Trees
+    Exec_DG_Refines
 begin
 
 section \<open>The executable equation generator and its transport\<close>
@@ -28,7 +28,7 @@ definition dg_cmb_at_of ::
      \<Rightarrow> (pp \<times> unit, unit, ('d, 'h) dg_state) strategy_tree"
 where
   "dg_cmb_at_of S ctx ca cc p =
-     map_gtree (\<lambda>_. ()) (map_ltree (\<lambda>w. (w, ctx))
+     relabel_gtree (\<lambda>_. ()) (relabel_ltree (\<lambda>w. (w, ctx))
        (dg_spec_combine_tree S (call_info_of ca p) cc (FunctionResult p)))"
 
 definition dg_cmb_of ::
@@ -46,7 +46,7 @@ definition dg_extra_of ::
 where
   "dg_extra_of S g route ctx v =
      map (\<lambda>(cl, ca).
-       map_gtree (\<lambda>_. ()) (map_ltree (\<lambda>w. (w, ctx))
+       relabel_gtree (\<lambda>_. ()) (relabel_ltree (\<lambda>w. (w, ctx))
          (dg_edge_tree (dgs_enter S (call_info_of ca (case v of FunctionEntry p \<Rightarrow> p | _ \<Rightarrow> undefined)))
             cl))) (entry_call_list g v)"
 
@@ -57,108 +57,6 @@ where
   "dg_gen_of S g bot0 s0d s0g =
      side_cfg_T_eff_keyed_seed_dg intra_predecessor_addr_list (\<lambda>_. ())
        (\<lambda>_ _ _ _. ()) (dg_cmb_of S g) (dg_extra_of S g) g S bot0 s0d s0g"
-
-subsection \<open>Side-effect commutation for the generator\<close>
-
-lemma sides_of_rhs_Inl_bot: "sides_of_rhs t \<sigma> (Inl a) = bot"
-  by (induction t arbitrary: \<sigma>) (auto simp: Let_def)
-
-
-lemma sides_dg_edge_tree_commute_for:
-  assumes H: "\<And>d g. map_prod (fun_of_exec_dg_st_for gs) (fun_of_exec_dg_st_for gs) (step_st d g) = step_abs (fun_of_exec_dg_st_for gs d) (fun_of_exec_dg_st_for gs g)"
-  shows "fun_of_dg_st_for gs (sides_of_rhs (dg_edge_tree step_st u) \<tau>_st k)
-       = sides_of_rhs (dg_edge_tree step_abs u) (fun_of_dg_st_for gs \<circ> \<tau>_st) k"
-proof (cases k)
-  case (Inr b)
-  have hg: "fst (step_abs (fun_of_exec_dg_st_for gs (locals (\<tau>_st (Inl u)))) (fun_of_exec_dg_st_for gs (globs (\<tau>_st (Inr ())))))
-        = fun_of_exec_dg_st_for gs (fst (step_st (locals (\<tau>_st (Inl u))) (globs (\<tau>_st (Inr ())))))"
-    using H[of "locals (\<tau>_st (Inl u))" "globs (\<tau>_st (Inr ()))"]
-    by (metis map_prod_simp fst_conv surj_pair)
-  show ?thesis using Inr
-    by (simp add: sides_dg_edge_tree_Inr fun_of_dg_st_for_def fun_of_resolved_st_q_for_bot hg o_def flip: bot_fun_def)
-next
-  case (Inl a)
-  show ?thesis using Inl
-    by (simp add: sides_dg_edge_tree_Inl fun_of_dg_st_for_bot)
-qed
-
-
-lemma sides_dg_combine_tree_commute_for:
-  assumes H: "\<And>dst dc de g. map_prod (fun_of_exec_dg_st_for gs) (fun_of_exec_dg_st_for gs) (comb_st dst dc de g)
-                        = comb_abs dst (fun_of_exec_dg_st_for gs dc) (fun_of_exec_dg_st_for gs de) (fun_of_exec_dg_st_for gs g)"
-  shows "fun_of_dg_st_for gs (sides_of_rhs (dg_combine_tree comb_st dst cc ex) \<tau>_st k)
-       = sides_of_rhs (dg_combine_tree comb_abs dst cc ex) (fun_of_dg_st_for gs \<circ> \<tau>_st) k"
-proof (cases k)
-  case (Inr b)
-  have hg: "fst (comb_abs dst (fun_of_exec_dg_st_for gs (locals (\<tau>_st (Inl cc)))) (fun_of_exec_dg_st_for gs (locals (\<tau>_st (Inl ex)))) (fun_of_exec_dg_st_for gs (globs (\<tau>_st (Inr ())))))
-        = fun_of_exec_dg_st_for gs (fst (comb_st dst (locals (\<tau>_st (Inl cc))) (locals (\<tau>_st (Inl ex))) (globs (\<tau>_st (Inr ())))))"
-    using H[of dst "locals (\<tau>_st (Inl cc))" "locals (\<tau>_st (Inl ex))" "globs (\<tau>_st (Inr ()))"]
-    by (metis map_prod_simp fst_conv surj_pair)
-  show ?thesis using Inr
-    by (simp add: sides_dg_combine_tree_Inr fun_of_dg_st_for_def fun_of_resolved_st_q_for_bot hg o_def flip: bot_fun_def)
-next
-  case (Inl a)
-  show ?thesis using Inl
-    by (simp add: dg_combine_tree_def fun_of_dg_st_for_bot)
-qed
-
-lemma sides_wrap_reduce:
-  "sides_of_rhs (map_gtree (\<lambda>_. gk) (map_ltree lk t)) \<sigma> (Inr gk)
-     = sides_of_rhs t (\<lambda>z. \<sigma> (map_sum lk (\<lambda>_. gk) z)) (Inr ())"
-  apply (subst sides_map_gtree_unit[where r="\<lambda>_. gk", simplified])
-  apply (subst sides_map_ltree_Inr)
-  apply (simp add: sum.map_comp o_def)
-  done
-
-
-lemma sides_wrapped_edge_commute_for:
-  assumes H: "\<And>d g. map_prod (fun_of_exec_dg_st_for gs) (fun_of_exec_dg_st_for gs) (step_st d g) = step_abs (fun_of_exec_dg_st_for gs d) (fun_of_exec_dg_st_for gs g)"
-  shows "fun_of_dg_st_for gs (sides_of_rhs (map_gtree (\<lambda>_. gk) (map_ltree lk (dg_edge_tree step_st u))) \<sigma>_st k)
-       = sides_of_rhs (map_gtree (\<lambda>_. gk) (map_ltree lk (dg_edge_tree step_abs u))) (fun_of_dg_st_for gs \<circ> \<sigma>_st) k"
-proof (cases k)
-  case (Inl a)
-  show ?thesis by (simp add: Inl sides_of_rhs_Inl_bot fun_of_dg_st_for_bot)
-next
-  case (Inr b)
-  show ?thesis
-  proof (cases "b = gk")
-    case True
-    have "fun_of_dg_st_for gs (sides_of_rhs (dg_edge_tree step_st u) (\<lambda>z. \<sigma>_st (map_sum lk (\<lambda>_. gk) z)) (Inr ()))
-        = sides_of_rhs (dg_edge_tree step_abs u) (fun_of_dg_st_for gs \<circ> (\<lambda>z. \<sigma>_st (map_sum lk (\<lambda>_. gk) z))) (Inr ())"
-      using H by (rule sides_dg_edge_tree_commute_for)
-    thus ?thesis by (simp add: Inr True sides_wrap_reduce o_def)
-  next
-    case False
-    hence nb: "b \<notin> range (\<lambda>_::unit. gk)" by simp
-    show ?thesis by (simp add: Inr sides_map_gtree_off[OF nb] fun_of_dg_st_for_bot)
-  qed
-qed
-
-
-lemma sides_wrapped_combine_commute_for:
-  assumes H: "\<And>dst dc de g. map_prod (fun_of_exec_dg_st_for gs) (fun_of_exec_dg_st_for gs) (comb_st dst dc de g)
-                        = comb_abs dst (fun_of_exec_dg_st_for gs dc) (fun_of_exec_dg_st_for gs de) (fun_of_exec_dg_st_for gs g)"
-  shows "fun_of_dg_st_for gs (sides_of_rhs (map_gtree (\<lambda>_. gk) (map_ltree lk (dg_combine_tree comb_st dst cc ex))) \<sigma>_st k)
-       = sides_of_rhs (map_gtree (\<lambda>_. gk) (map_ltree lk (dg_combine_tree comb_abs dst cc ex))) (fun_of_dg_st_for gs \<circ> \<sigma>_st) k"
-proof (cases k)
-  case (Inl a)
-  show ?thesis by (simp add: Inl sides_of_rhs_Inl_bot fun_of_dg_st_for_bot)
-next
-  case (Inr b)
-  show ?thesis
-  proof (cases "b = gk")
-    case True
-    have "fun_of_dg_st_for gs (sides_of_rhs (dg_combine_tree comb_st dst cc ex) (\<lambda>z. \<sigma>_st (map_sum lk (\<lambda>_. gk) z)) (Inr ()))
-        = sides_of_rhs (dg_combine_tree comb_abs dst cc ex) (fun_of_dg_st_for gs \<circ> (\<lambda>z. \<sigma>_st (map_sum lk (\<lambda>_. gk) z))) (Inr ())"
-      using H by (rule sides_dg_combine_tree_commute_for)
-    thus ?thesis by (simp add: Inr True sides_wrap_reduce o_def)
-  next
-    case False
-    hence nb: "b \<notin> range (\<lambda>_::unit. gk)" by simp
-    show ?thesis by (simp add: Inr sides_map_gtree_off[OF nb] fun_of_dg_st_for_bot)
-  qed
-qed
-
 
 subsection \<open>Dependency commutation for the generator\<close>
 
@@ -171,25 +69,8 @@ text \<open>
 lemma dep_aux_dg_edge_tree: "dep_aux \<sigma> (dg_edge_tree step u) = {Inl u, Inr ()}"
   by (simp add: dg_edge_tree_def dep_aux_def)
 
-lemma dep_aux_dg_combine_tree: "dep_aux \<sigma> (dg_combine_tree comb dst cc ex) = {Inl cc, Inl ex, Inr ()}"
-  by (auto simp: dg_combine_tree_def dep_aux_def)
-
 lemma dep_aux_Side: "dep_aux \<sigma> (Side y d t) = dep_aux \<sigma> t"
   by (simp add: dep_aux_def)
-
-lemma dep_aux_map_gtree:
-  "dep_aux \<sigma> (map_gtree r t) = map_sum id r ` dep_aux (\<lambda>z. \<sigma> (map_sum id r z)) t"
-  by (induction t arbitrary: \<sigma>) (auto simp: dep_aux_def)
-
-lemma dep_aux_wrapped_edge_eq:
-  "dep_aux \<sigma>_st (map_gtree (\<lambda>_. gk) (map_ltree lk (dg_edge_tree step_st u)))
-     = dep_aux \<sigma>_abs (map_gtree (\<lambda>_. gk) (map_ltree lk (dg_edge_tree step_abs u)))"
-  by (simp add: dep_aux_map_gtree dep_aux_map_ltree dep_aux_dg_edge_tree)
-
-lemma dep_aux_wrapped_combine_eq:
-  "dep_aux \<sigma>_st (map_gtree (\<lambda>_. gk) (map_ltree lk (dg_combine_tree comb_st dst cc ex)))
-     = dep_aux \<sigma>_abs (map_gtree (\<lambda>_. gk) (map_ltree lk (dg_combine_tree comb_abs dst cc ex)))"
-  by (simp add: dep_aux_map_gtree dep_aux_map_ltree dep_aux_dg_combine_tree)
 
 lemma dep_aux_side_rhs_fold_dg_commute:
   assumes "list_all2 (\<lambda>t_st t_abs. dep_aux \<sigma>_st t_st = dep_aux \<sigma>_abs t_abs) ts_st ts_abs"
@@ -206,60 +87,6 @@ next
     by (rule Cons.IH)
   show ?case by (simp add: dep_aux_seqcomp hd ih)
 qed
-
-subsection \<open>Classifier-parametric fold transport\<close>
-
-text \<open>
-  Fold-commute lemmas reading through the generic \<open>fun_of_exec_dg_st_for gs\<close>/
-  \<open>fun_of_dg_st_for gs\<close> readback.  \<open>dep_aux_side_rhs_fold_dg_commute\<close> already
-  never mentions a readback, so it transports unchanged.
-\<close>
-
-lemma side_acc_dg_commute_for:
-  assumes "list_all2 (\<lambda>t_st t_abs.
-             fun_of_dg_st_for gs (traverse_rhs t_st \<sigma>_st) = traverse_rhs t_abs (fun_of_dg_st_for gs \<circ> \<sigma>_st))
-           ts_st ts_abs"
-  shows "fun_of_exec_dg_st_for gs (side_acc_dg acc_st \<sigma>_st ts_st)
-           = side_acc_dg (fun_of_exec_dg_st_for gs acc_st) (fun_of_dg_st_for gs \<circ> \<sigma>_st) ts_abs"
-  using assms
-proof (induction ts_st ts_abs arbitrary: acc_st rule: list_all2_induct)
-  case Nil
-  thus ?case by simp
-next
-  case (Cons t_st ts_st t_abs ts_abs)
-  have hl: "fun_of_exec_dg_st_for gs (locals (traverse_rhs t_st \<sigma>_st))
-              = locals (traverse_rhs t_abs (fun_of_dg_st_for gs \<circ> \<sigma>_st))"
-    using Cons.hyps(1) by (metis fun_of_dg_st_for_simps(1))
-  have h: "fun_of_exec_dg_st_for gs (acc_st \<squnion> locals (traverse_rhs t_st \<sigma>_st))
-           = fun_of_exec_dg_st_for gs acc_st \<squnion> locals (traverse_rhs t_abs (fun_of_dg_st_for gs \<circ> \<sigma>_st))"
-    unfolding fun_of_exec_dg_st_for_def
-    by (simp add: fun_of_resolved_st_q_for_sup hl[unfolded fun_of_exec_dg_st_for_def])
-  show ?case
-    by (metis (no_types, lifting) Cons.IH h side_acc_dg.simps(2))
-qed
-
-lemma sides_side_rhs_fold_dg_commute_for:
-  assumes "list_all2 (\<lambda>t_st t_abs.
-             fun_of_dg_st_for gs (traverse_rhs t_st \<sigma>_st) = traverse_rhs t_abs (fun_of_dg_st_for gs \<circ> \<sigma>_st)
-             \<and> (\<forall>k. fun_of_dg_st_for gs (sides_of_rhs t_st \<sigma>_st k) = sides_of_rhs t_abs (fun_of_dg_st_for gs \<circ> \<sigma>_st) k))
-           ts_st ts_abs"
-  shows "fun_of_dg_st_for gs (sides_of_rhs (side_rhs_fold_dg acc_st ts_st) \<sigma>_st k)
-           = sides_of_rhs (side_rhs_fold_dg acc_abs ts_abs) (fun_of_dg_st_for gs \<circ> \<sigma>_st) k"
-  using assms
-proof (induction ts_st ts_abs arbitrary: acc_st acc_abs rule: list_all2_induct)
-  case Nil
-  thus ?case by (simp add: fun_of_dg_st_for_bot bot_fun_def)
-next
-  case (Cons t_st ts_st t_abs ts_abs)
-  have sd: "fun_of_dg_st_for gs (sides_of_rhs t_st \<sigma>_st k) = sides_of_rhs t_abs (fun_of_dg_st_for gs \<circ> \<sigma>_st) k"
-    using Cons.hyps(1) by simp
-  have ih: "fun_of_dg_st_for gs (sides_of_rhs (side_rhs_fold_dg (acc_st \<squnion> locals (traverse_rhs t_st \<sigma>_st)) ts_st) \<sigma>_st k)
-          = sides_of_rhs (side_rhs_fold_dg (acc_abs \<squnion> locals (traverse_rhs t_abs (fun_of_dg_st_for gs \<circ> \<sigma>_st))) ts_abs) (fun_of_dg_st_for gs \<circ> \<sigma>_st) k"
-    by (rule Cons.IH)
-  show ?case
-    by (simp add: sides_of_rhs_seqcomp fun_of_dg_st_for_sup sd ih comp_def)
-qed
-
 
 subsection \<open>Carrier-generic whole-CFG commute\<close>
 
@@ -311,74 +138,6 @@ lemma fun_of_dg_st_gen_mono:
   "(a :: ('a,'b) dg_state) \<le> b \<Longrightarrow> fun_of_dg_st_gen Floc Fglob a \<le> fun_of_dg_st_gen Floc Fglob b"
   by (auto simp: less_eq_dg_state_def Floc_mono Fglob_mono)
 
-subsubsection \<open>Per-tree traversal commutation\<close>
-
-lemma traverse_dg_edge_tree_commute:
-  assumes H: "\<And>d g. map_prod Fglob Floc (step_st d g) = step_abs (Floc d) (Fglob g)"
-  shows "fun_of_dg_st_gen Floc Fglob (traverse_rhs (dg_edge_tree step_st u) \<sigma>_st)
-           = traverse_rhs (dg_edge_tree step_abs u) (fun_of_dg_st_gen Floc Fglob \<circ> \<sigma>_st)"
-proof -
-  have "snd (step_abs (Floc (locals (\<sigma>_st (Inl u)))) (Fglob (globs (\<sigma>_st (Inr ())))))
-        = Floc (snd (step_st (locals (\<sigma>_st (Inl u))) (globs (\<sigma>_st (Inr ())))))"
-    using H[of "locals (\<sigma>_st (Inl u))" "globs (\<sigma>_st (Inr ()))"]
-    by (metis map_prod_simp snd_conv surj_pair)
-  thus ?thesis
-    by (simp add: traverse_dg_edge_tree Fglob_bot)
-qed
-
-lemma traverse_wrapped_edge_commute:
-  assumes H: "\<And>d g. map_prod Fglob Floc (step_st d g) = step_abs (Floc d) (Fglob g)"
-  shows "fun_of_dg_st_gen Floc Fglob (traverse_rhs (map_gtree (\<lambda>_. gk) (map_ltree lk (dg_edge_tree step_st u))) \<sigma>_st)
-       = traverse_rhs (map_gtree (\<lambda>_. gk) (map_ltree lk (dg_edge_tree step_abs u))) (fun_of_dg_st_gen Floc Fglob \<circ> \<sigma>_st)"
-proof -
-  have "fun_of_dg_st_gen Floc Fglob (traverse_rhs (dg_edge_tree step_st u) (\<lambda>z. \<sigma>_st (map_sum lk (\<lambda>_. gk) z)))
-        = traverse_rhs (dg_edge_tree step_abs u) (fun_of_dg_st_gen Floc Fglob \<circ> (\<lambda>z. \<sigma>_st (map_sum lk (\<lambda>_. gk) z)))"
-    using H by (rule traverse_dg_edge_tree_commute)
-  thus ?thesis
-    by (simp add: traverse_rhs_map_gtree traverse_rhs_map_ltree sum.map_comp comp_def o_def)
-qed
-
-lemma sides_dg_edge_tree_commute:
-  assumes H: "\<And>d g. map_prod Fglob Floc (step_st d g) = step_abs (Floc d) (Fglob g)"
-  shows "fun_of_dg_st_gen Floc Fglob (sides_of_rhs (dg_edge_tree step_st u) \<tau>_st k)
-       = sides_of_rhs (dg_edge_tree step_abs u) (fun_of_dg_st_gen Floc Fglob \<circ> \<tau>_st) k"
-proof (cases k)
-  case (Inr b)
-  have hg: "fst (step_abs (Floc (locals (\<tau>_st (Inl u)))) (Fglob (globs (\<tau>_st (Inr ())))))
-        = Fglob (fst (step_st (locals (\<tau>_st (Inl u))) (globs (\<tau>_st (Inr ())))))"
-    using H[of "locals (\<tau>_st (Inl u))" "globs (\<tau>_st (Inr ()))"]
-    by (metis map_prod_simp fst_conv surj_pair)
-  show ?thesis using Inr
-    by (simp add: sides_dg_edge_tree_Inr Floc_bot hg o_def)
-next
-  case (Inl a)
-  show ?thesis using Inl
-    by (simp add: sides_dg_edge_tree_Inl)
-qed
-
-lemma sides_wrapped_edge_commute:
-  assumes H: "\<And>d g. map_prod Fglob Floc (step_st d g) = step_abs (Floc d) (Fglob g)"
-  shows "fun_of_dg_st_gen Floc Fglob (sides_of_rhs (map_gtree (\<lambda>_. gk) (map_ltree lk (dg_edge_tree step_st u))) \<sigma>_st k)
-       = sides_of_rhs (map_gtree (\<lambda>_. gk) (map_ltree lk (dg_edge_tree step_abs u))) (fun_of_dg_st_gen Floc Fglob \<circ> \<sigma>_st) k"
-proof (cases k)
-  case (Inl a)
-  show ?thesis by (simp add: Inl sides_of_rhs_Inl_bot)
-next
-  case (Inr b)
-  show ?thesis
-  proof (cases "b = gk")
-    case True
-    have "fun_of_dg_st_gen Floc Fglob (sides_of_rhs (dg_edge_tree step_st u) (\<lambda>z. \<sigma>_st (map_sum lk (\<lambda>_. gk) z)) (Inr ()))
-        = sides_of_rhs (dg_edge_tree step_abs u) (fun_of_dg_st_gen Floc Fglob \<circ> (\<lambda>z. \<sigma>_st (map_sum lk (\<lambda>_. gk) z))) (Inr ())"
-      using H by (rule sides_dg_edge_tree_commute)
-    thus ?thesis by (simp add: Inr True sides_wrap_reduce o_def)
-  next
-    case False
-    hence nb: "b \<notin> range (\<lambda>_::unit. gk)" by simp
-    show ?thesis by (simp add: Inr sides_map_gtree_off[OF nb])
-  qed
-qed
-
 subsubsection \<open>Bundled per-tree transport relation\<close>
 
 definition dg_tree_st_commute ::
@@ -421,17 +180,6 @@ lemma dg_list_commute_dep:
   "list_all2 (dg_tree_st_commute \<sigma>_st) ts_st ts_abs
      \<Longrightarrow> list_all2 (\<lambda>t_st t_abs. dep_aux \<sigma>_st t_st = dep_aux (fun_of_dg_st_gen Floc Fglob \<circ> \<sigma>_st) t_abs) ts_st ts_abs"
   by (erule list_all2_mono) (simp add: dg_tree_st_commute_def)
-
-lemma dg_tree_st_commute_wrapped_edge:
-  assumes H: "\<And>d g. map_prod Fglob Floc (step_st d g) = step_abs (Floc d) (Fglob g)"
-  shows "dg_tree_st_commute \<sigma>_st
-           (map_gtree (\<lambda>_. gk) (map_ltree lk (dg_edge_tree step_st u)))
-           (map_gtree (\<lambda>_. gk) (map_ltree lk (dg_edge_tree step_abs u)))"
-  unfolding dg_tree_st_commute_def
-  by (intro conjI allI
-        traverse_wrapped_edge_commute[where step_st=step_st and step_abs=step_abs, OF H]
-        sides_wrapped_edge_commute[where step_st=step_st and step_abs=step_abs, OF H]
-        dep_aux_wrapped_edge_eq)
 
 text \<open>The same transport at an address-formed edge tree: the source is read through the
   valuation either way, so only the published key needs a case distinction.\<close>
@@ -476,114 +224,6 @@ lemma dg_tree_st_commute_at_edge:
         traverse_dg_edge_tree_at_commute[where step_st=step_st and step_abs=step_abs, OF H]
         sides_dg_edge_tree_at_commute[where step_st=step_st and step_abs=step_abs, OF H])
      (simp add: dep_aux_dg_edge_tree_at)
-
-subsubsection \<open>Combine-tree transport, generic in the reader\<close>
-
-text \<open>
-  The combine-tree analogue of \<open>traverse_dg_edge_tree_commute\<close>/\<open>sides_dg_edge_tree_commute\<close>
-  above, factored generically here rather than duplicated per reader: the diagonal
-  (\<open>fun_of_exec_dg_st_for gs\<close>) and lifted (\<open>map_lift (fun_of_exec_dg_st_for gs)\<close>) instances
-  both cite these directly, so only the \<open>dg_cmb_of\<close>-specific instantiation below is
-  reader-specific, not the tree-structure reasoning itself.
-\<close>
-
-lemma traverse_dg_combine_tree_commute:
-  assumes H: "\<And>dst dc de g. map_prod Fglob Floc (comb_st dst dc de g)
-                        = comb_abs dst (Floc dc) (Floc de) (Fglob g)"
-  shows "fun_of_dg_st_gen Floc Fglob (traverse_rhs (dg_combine_tree comb_st dst cc ex) \<sigma>_st)
-           = traverse_rhs (dg_combine_tree comb_abs dst cc ex) (fun_of_dg_st_gen Floc Fglob \<circ> \<sigma>_st)"
-proof -
-  have "snd (comb_abs dst (Floc (locals (\<sigma>_st (Inl cc)))) (Floc (locals (\<sigma>_st (Inl ex))))
-              (Fglob (globs (\<sigma>_st (Inr ())))))
-        = Floc (snd (comb_st dst (locals (\<sigma>_st (Inl cc))) (locals (\<sigma>_st (Inl ex)))
-              (globs (\<sigma>_st (Inr ())))))"
-    using H[of dst "locals (\<sigma>_st (Inl cc))" "locals (\<sigma>_st (Inl ex))" "globs (\<sigma>_st (Inr ()))"]
-    by (metis map_prod_simp snd_conv surj_pair)
-  thus ?thesis
-    by (simp add: traverse_dg_combine_tree Fglob_bot)
-qed
-
-lemma traverse_wrapped_combine_commute:
-  assumes H: "\<And>dst dc de g. map_prod Fglob Floc (comb_st dst dc de g)
-                        = comb_abs dst (Floc dc) (Floc de) (Fglob g)"
-  shows "fun_of_dg_st_gen Floc Fglob (traverse_rhs (map_gtree gk (map_ltree lk (dg_combine_tree comb_st dst cc ex))) \<sigma>_st)
-       = traverse_rhs (map_gtree gk (map_ltree lk (dg_combine_tree comb_abs dst cc ex))) (fun_of_dg_st_gen Floc Fglob \<circ> \<sigma>_st)"
-proof -
-  have "fun_of_dg_st_gen Floc Fglob (traverse_rhs (dg_combine_tree comb_st dst cc ex) (\<lambda>z. \<sigma>_st (map_sum lk gk z)))
-        = traverse_rhs (dg_combine_tree comb_abs dst cc ex) (fun_of_dg_st_gen Floc Fglob \<circ> (\<lambda>z. \<sigma>_st (map_sum lk gk z)))"
-    using H by (rule traverse_dg_combine_tree_commute)
-  thus ?thesis
-    by (simp add: traverse_rhs_map_gtree traverse_rhs_map_ltree sum.map_comp comp_def o_def)
-qed
-
-lemma sides_dg_combine_tree_commute:
-  assumes H: "\<And>dst dc de g. map_prod Fglob Floc (comb_st dst dc de g)
-                        = comb_abs dst (Floc dc) (Floc de) (Fglob g)"
-  shows "fun_of_dg_st_gen Floc Fglob (sides_of_rhs (dg_combine_tree comb_st dst cc ex) \<tau>_st k)
-       = sides_of_rhs (dg_combine_tree comb_abs dst cc ex) (fun_of_dg_st_gen Floc Fglob \<circ> \<tau>_st) k"
-proof (cases k)
-  case (Inr b)
-  have hg: "fst (comb_abs dst (Floc (locals (\<tau>_st (Inl cc)))) (Floc (locals (\<tau>_st (Inl ex)))) (Fglob (globs (\<tau>_st (Inr ())))))
-        = Fglob (fst (comb_st dst (locals (\<tau>_st (Inl cc))) (locals (\<tau>_st (Inl ex))) (globs (\<tau>_st (Inr ())))))"
-    using H[of dst "locals (\<tau>_st (Inl cc))" "locals (\<tau>_st (Inl ex))" "globs (\<tau>_st (Inr ()))"]
-    by (metis map_prod_simp fst_conv surj_pair)
-  show ?thesis using Inr
-    by (simp add: sides_dg_combine_tree_Inr Floc_bot hg o_def)
-next
-  case (Inl a)
-  show ?thesis using Inl
-    by (simp add: dg_combine_tree_def fun_of_dg_st_gen_bot)
-qed
-
-lemma sides_wrapped_combine_commute:
-  assumes H: "\<And>dst dc de g. map_prod Fglob Floc (comb_st dst dc de g)
-                        = comb_abs dst (Floc dc) (Floc de) (Fglob g)"
-  shows "fun_of_dg_st_gen Floc Fglob (sides_of_rhs (map_gtree (\<lambda>_. gk) (map_ltree lk (dg_combine_tree comb_st dst cc ex))) \<sigma>_st k)
-       = sides_of_rhs (map_gtree (\<lambda>_. gk) (map_ltree lk (dg_combine_tree comb_abs dst cc ex))) (fun_of_dg_st_gen Floc Fglob \<circ> \<sigma>_st) k"
-proof (cases k)
-  case (Inl a)
-  show ?thesis by (simp add: Inl sides_of_rhs_Inl_bot)
-next
-  case (Inr b)
-  show ?thesis
-  proof (cases "b = gk")
-    case True
-    have "fun_of_dg_st_gen Floc Fglob (sides_of_rhs (dg_combine_tree comb_st dst cc ex) (\<lambda>z. \<sigma>_st (map_sum lk (\<lambda>_. gk) z)) (Inr ()))
-        = sides_of_rhs (dg_combine_tree comb_abs dst cc ex) (fun_of_dg_st_gen Floc Fglob \<circ> (\<lambda>z. \<sigma>_st (map_sum lk (\<lambda>_. gk) z))) (Inr ())"
-      using H by (rule sides_dg_combine_tree_commute)
-    thus ?thesis by (simp add: Inr True sides_wrap_reduce o_def)
-  next
-    case False
-    hence nb: "b \<notin> range (\<lambda>_::unit. gk)" by simp
-    show ?thesis by (simp add: Inr sides_map_gtree_off[OF nb])
-  qed
-qed
-
-lemma dg_tree_st_commute_wrapped_combine:
-  assumes H: "\<And>dst dc de g. map_prod Fglob Floc (comb_st dst dc de g)
-                        = comb_abs dst (Floc dc) (Floc de) (Fglob g)"
-  shows "dg_tree_st_commute \<sigma>_st
-           (map_gtree (\<lambda>_. gk) (map_ltree lk (dg_combine_tree comb_st dst cc ex)))
-           (map_gtree (\<lambda>_. gk) (map_ltree lk (dg_combine_tree comb_abs dst cc ex)))"
-  unfolding dg_tree_st_commute_def
-proof (intro conjI)
-  show "fun_of_dg_st_gen Floc Fglob (traverse_rhs (map_gtree (\<lambda>_. gk) (map_ltree lk (dg_combine_tree comb_st dst cc ex))) \<sigma>_st)
-          = traverse_rhs (map_gtree (\<lambda>_. gk) (map_ltree lk (dg_combine_tree comb_abs dst cc ex))) (fun_of_dg_st_gen Floc Fglob \<circ> \<sigma>_st)"
-    by (rule traverse_wrapped_combine_commute[where comb_st=comb_st and comb_abs=comb_abs, OF H])
-next
-  show "\<forall>k. fun_of_dg_st_gen Floc Fglob (sides_of_rhs (map_gtree (\<lambda>_. gk) (map_ltree lk (dg_combine_tree comb_st dst cc ex))) \<sigma>_st k)
-          = sides_of_rhs (map_gtree (\<lambda>_. gk) (map_ltree lk (dg_combine_tree comb_abs dst cc ex))) (fun_of_dg_st_gen Floc Fglob \<circ> \<sigma>_st) k"
-  proof
-    fix k
-    show "fun_of_dg_st_gen Floc Fglob (sides_of_rhs (map_gtree (\<lambda>_. gk) (map_ltree lk (dg_combine_tree comb_st dst cc ex))) \<sigma>_st k)
-            = sides_of_rhs (map_gtree (\<lambda>_. gk) (map_ltree lk (dg_combine_tree comb_abs dst cc ex))) (fun_of_dg_st_gen Floc Fglob \<circ> \<sigma>_st) k"
-      by (rule sides_wrapped_combine_commute[where comb_st=comb_st and comb_abs=comb_abs, OF H])
-  qed
-next
-  show "dep_aux \<sigma>_st (map_gtree (\<lambda>_. gk) (map_ltree lk (dg_combine_tree comb_st dst cc ex)))
-          = dep_aux (fun_of_dg_st_gen Floc Fglob \<circ> \<sigma>_st) (map_gtree (\<lambda>_. gk) (map_ltree lk (dg_combine_tree comb_abs dst cc ex)))"
-    by (rule dep_aux_wrapped_combine_eq)
-qed
 
 end
 
@@ -1006,3 +646,4 @@ lemma dg_tree_st_commute_routed_extra_g:
 end
 
 end
+
